PivotBetree/BucketGenerator.i.dfy
@@ -1,0 +1,461 @@
+include "BucketIterator.i.dfy"
+//
+// A mathematical description of bucket generators.
+// It's like an iterator, but it doesn't directly refer to an actual bucket.
+// The bucket may be implicit.
+//
+
+module BucketGenerator {
+  import opened Options
+  import opened Maps
+  import opened BucketsLib
+  import opened PivotsLib
+  import opened ValueMessage
+  import opened Sequences
+  import opened BucketIterator
+  import UI
+
+  datatype Generator =
+    | BasicGenerator(
+        bucket: Bucket,
+        it: Iterator
+      )
+    | ComposeGenerator(
+        top: Generator,
+        bot: Generator,
+        next: IteratorOutput
+      )
+
+  predicate WF(g: Generator)
+  {
+    && (g.BasicGenerator? ==> (
+      && WFIter(g.bucket, g.it)
+    ))
+    && (g.ComposeGenerator? ==> (
+      && WF(g.top)
+      && WF(g.bot)
+    ))
+  }
+
+  function GenLeft(g: Generator) : (next : IteratorOutput)
+  {
+    match g {
+      case BasicGenerator(bucket, it) => (
+        g.it.next
+      )
+      case ComposeGenerator(top, bot, next) => (
+        g.next
+      )
+    }
+  }
+
+  function {:opaque} BasicGenPop(g: Generator) : (g' : Generator)
+  requires WF(g)
+  requires GenLeft(g).Next?
+  requires g.BasicGenerator?
+  decreases g, 0
+  ensures WF(g')
+  {
+    BasicGenerator(
+      g.bucket,
+      IterInc(g.bucket, g.it))
+  }
+
+  function {:opaque} MergeGenPop(g: Generator) : (g' : Generator)
+  requires WF(g)
+  requires GenLeft(g).Next?
+  requires g.ComposeGenerator?
+  decreases g, 0
+  ensures WF(g')
+  {
+    var top := g.top;
+    var bot := g.bot;
+    if GenLeft(top).Next? && GenLeft(bot).Next?
+        && GenLeft(top).key == GenLeft(bot).key then (
+      ComposeGenerator(
+        GenPop(top),
+        GenPop(bot),
+        Next(GenLeft(top).key,
+            Merge(GenLeft(top).msg, GenLeft(bot).msg)))
+    ) else if GenLeft(top).Next?
+        && (GenLeft(bot).Next? ==> Keyspace.lt(GenLeft(top).key, GenLeft(bot).key)) then (
+      ComposeGenerator(
+        GenPop(top),
+        bot,
+        GenLeft(top))
+    ) else if GenLeft(bot).Next? then (
+      ComposeGenerator(
+        top,
+        GenPop(bot),
+        GenLeft(bot))
+    ) else (
+      ComposeGenerator(
+        top,
+        bot,
+        Done)
+    )
+  }
+
+  function {:opaque} GenPop(g: Generator) : (g' : Generator)
+  requires WF(g)
+  requires GenLeft(g).Next?
+  decreases g, 1
+  ensures WF(g')
+  {
+    match g {
+      case BasicGenerator(bucket, it) => (
+        BasicGenPop(g)
+      )
+      case ComposeGenerator(top, bot, next) => (
+        MergeGenPop(g)
+      )
+    }
+  }
+
+  function {:opaque} GenCompose(top: Generator, bot: Generator) : (g' : Generator)
+  requires WF(top)
+  requires WF(bot)
+  ensures WF(g')
+  {
+    // Yeah this is basically duplicated with the above, but when I tried to factor
+    // it out, I ran into weird interactions with decreases clauses.
+
+    if GenLeft(top).Next? && GenLeft(bot).Next?
+        && GenLeft(top).key == GenLeft(bot).key then (
+      ComposeGenerator(
+        GenPop(top),
+        GenPop(bot),
+        Next(GenLeft(top).key,
+            Merge(GenLeft(top).msg, GenLeft(bot).msg)))
+    ) else if GenLeft(top).Next?
+        && (GenLeft(bot).Next? ==> Keyspace.lt(GenLeft(top).key, GenLeft(bot).key)) then (
+      ComposeGenerator(
+        GenPop(top),
+        bot,
+        GenLeft(top))
+    ) else if GenLeft(bot).Next? then (
+      ComposeGenerator(
+        top,
+        GenPop(bot),
+        GenLeft(bot))
+    ) else (
+      ComposeGenerator(
+        top,
+        bot,
+        Done)
+    )
+  }
+
+  function {:opaque} GenFromBucketWithLowerBound(bucket: Bucket, start: UI.RangeStart) : (g : Generator)
+  ensures WF(g)
+  {
+    var it := match start {
+      case SExclusive(key) => IterFindFirstGt(bucket, key)
+      case SInclusive(key) => IterFindFirstGte(bucket, key)
+      case NegativeInf => IterStart(bucket)
+    };
+    BasicGenerator(bucket, it)
+  }
+
+  function {:opaque} GenFromBucketStackWithLowerBound(buckets: seq<Bucket>, start: UI.RangeStart) : (g : Generator)
+  requires |buckets| >= 1
+  decreases |buckets|
+  ensures WF(g)
+  {
+    if |buckets| == 1 then (
+      GenFromBucketWithLowerBound(buckets[0], start)
+    ) else (
+      var mid := |buckets| / 2;
+      GenCompose(
+        GenFromBucketStackWithLowerBound(buckets[..mid], start),
+        GenFromBucketStackWithLowerBound(buckets[mid..], start)
+      )
+    )
+  }
+
+  // Characterizing what the generators return
+
+  protected predicate Monotonic(g: Generator)
+  {
+    g.ComposeGenerator? ==> (
+      && (g.next.Next? && GenLeft(g.top).Next? ==> Keyspace.lt(g.next.key, GenLeft(g.top).key))
+      && (g.next.Next? && GenLeft(g.bot).Next? ==> Keyspace.lt(g.next.key, GenLeft(g.bot).key))
+      && (g.next.Done? ==> GenLeft(g.top).Done?)
+      && (g.next.Done? ==> GenLeft(g.bot).Done?)
+      && Monotonic(g.top)
+      && Monotonic(g.bot)
+    )
+  }
+
+  function {:opaque} BucketOf(g: Generator) : Bucket
+  {
+    match g {
+      case BasicGenerator(bucket, it) =>
+        if it.next.Done? then map[]
+        else map k | k in bucket && Keyspace.lte(it.next.key, k) :: bucket[k]
+      case ComposeGenerator(top, bot, next) =>
+        if next.Done? then map[]
+        else Compose(BucketOf(top), BucketOf(bot))[next.key := next.msg]
+    }
+  }
+
+  lemma reveal_BucketOf_for_Merge(g: Generator)
+  ensures g.ComposeGenerator? && g.next.Done? ==> BucketOf(g) == map[]
+  ensures g.ComposeGenerator? && g.next.Next? ==> BucketOf(g) ==
+        Compose(BucketOf(g.top), BucketOf(g.bot))[g.next.key := g.next.msg]
+  {
+    reveal_BucketOf();
+  }
+
+  predicate YieldsSortedBucket(g: Generator, b: Bucket)
+  {
+    && WF(g)
+    && Monotonic(g)
+    && BucketOf(g) == b
+  }
+
+  lemma GenLeftIsMinimum(g: Generator)
+  requires WF(g)
+  requires Monotonic(g)
+  ensures GenLeft(g).Done? ==> BucketOf(g) == map[]
+  ensures GenLeft(g).Next? ==> Keyspace.minimumOpt(BucketOf(g).Keys) == Some(GenLeft(g).key)
+  ensures GenLeft(g).Next? ==> BucketOf(g)[GenLeft(g).key] == GenLeft(g).msg
+  {
+    reveal_BucketOf();
+    if GenLeft(g).Next? {
+      if g.ComposeGenerator? {
+        reveal_Compose();
+        GenLeftIsMinimum(g.top);
+        GenLeftIsMinimum(g.bot);
+        assert GenLeft(g).key in BucketOf(g);
+        assert forall k | k in BucketOf(g) :: Keyspace.lte(GenLeft(g).key, k);
+        assert Keyspace.minimumOpt(BucketOf(g).Keys) == Some(GenLeft(g).key);
+      } else {
+        assert GenLeft(g).key in BucketOf(g);
+        assert forall k | k in BucketOf(g) :: Keyspace.lte(GenLeft(g).key, k);
+        assert Keyspace.minimumOpt(BucketOf(g).Keys) == Some(GenLeft(g).key);
+      }
+    }
+  }
+
+  lemma GenPopIsRemove(g: Generator)
+  requires WF(g)
+  requires Monotonic(g)
+  requires GenLeft(g).Next?
+  ensures |BucketOf(g).Keys| >= 1
+  ensures YieldsSortedBucket(GenPop(g),
+      MapRemove1(BucketOf(g), Keyspace.minimum(BucketOf(g).Keys)))
+  {
+    reveal_BucketOf();
+    var g' := GenPop(g);
+
+    GenLeftIsMinimum(g);
+    reveal_GenPop();
+
+    if g.BasicGenerator? {
+      reveal_BasicGenPop();
+      IterIncKeyGreater(g.bucket, g.it);
+
+      var b1 := BucketOf(g');
+      var b2 := MapRemove1(BucketOf(g), Keyspace.minimum(BucketOf(g).Keys));
+      forall k | k in b1 ensures k in b2 && b1[k] == b2[k]
+      {
+      }
+      forall k | k in b2 ensures k in b1
+      {
+        noKeyBetweenIterAndIterInc(g.bucket, g.it, k);
+      }
+      assert b1 == b2;
+    } else {
+      reveal_Compose();
+      reveal_MergeGenPop();
+
+      GenLeftIsMinimum(g.top);
+      GenLeftIsMinimum(g.bot);
+
+      if (GenLeft(g.top).Next?) {
+        GenPopIsRemove(g.top);
+        assert GenLeft(g.top).key in BucketOf(g.top).Keys;
+      }
+      if (GenLeft(g.bot).Next?) {
+        GenPopIsRemove(g.bot);
+        assert GenLeft(g.bot).key in BucketOf(g.bot).Keys;
+      }
+      assert YieldsSortedBucket(GenPop(g),
+        MapRemove1(BucketOf(g), Keyspace.minimum(BucketOf(g).Keys)));
+    }
+  }
+
+  lemma GenComposeIsMonotonic(top: Generator, bot: Generator)
+  requires WF(top)
+  requires WF(bot)
+  requires Monotonic(top)
+  requires Monotonic(bot)
+  ensures Monotonic(GenCompose(top, bot))
+  {
+    GenLeftIsMinimum(top);
+    GenLeftIsMinimum(bot);
+    reveal_BucketOf();
+
+    reveal_GenCompose();
+    if (GenLeft(top).Next?) {
+      GenPopIsRemove(top);
+      assert GenLeft(top).key in BucketOf(top).Keys;
+    }
+    if (GenLeft(bot).Next?) {
+      GenPopIsRemove(bot);
+      assert GenLeft(bot).key in BucketOf(bot).Keys;
+    }
+  }
+
+  lemma GenComposeIsCompose(top: Generator, bot: Generator)
+  requires WF(top)
+  requires WF(bot)
+  requires Monotonic(top)
+  requires Monotonic(bot)
+  ensures YieldsSortedBucket(GenCompose(top, bot), Compose(BucketOf(top), BucketOf(bot)))
+  {
+    var g := GenCompose(top, bot);
+
+    GenComposeIsMonotonic(top, bot);
+    reveal_Compose();
+    reveal_GenCompose();
+
+    GenLeftIsMinimum(top);
+    GenLeftIsMinimum(bot);
+
+    if (GenLeft(top).Next?) {
+      GenPopIsRemove(top);
+    }
+    if (GenLeft(bot).Next?) {
+      GenPopIsRemove(bot);
+    }
+
+    // Calling reveal_BucketOf() causes a trigger-loop for some reason
+    reveal_BucketOf_for_Merge(g);
+
+    /*if GenLeft(top).Next? && GenLeft(bot).Next?
+        && GenLeft(top).key == GenLeft(bot).key {
+      assert BucketOf(g)
+          == Compose(BucketOf(top), BucketOf(bot));
+    } else if GenLeft(top).Next?
+        && (GenLeft(bot).Next? ==> Keyspace.lt(GenLeft(top).key, GenLeft(bot).key)) {
+      assert BucketOf(g)
+          == Compose(BucketOf(GenPop(top)), BucketOf(bot))
+                [GenLeft(top).key := GenLeft(top).msg]
+          == Compose(MapRemove1(BucketOf(top), GenLeft(top).key), BucketOf(bot))
+                [GenLeft(top).key := GenLeft(top).msg]
+          == Compose(BucketOf(top), BucketOf(bot));
+    } else if GenLeft(bot).Next? {
+      assert BucketOf(g)
+          == Compose(BucketOf(top), MapRemove1(BucketOf(bot), GenLeft(bot).key))
+                [GenLeft(bot).key := GenLeft(bot).msg]
+          == Compose(BucketOf(top), BucketOf(bot));
+    } else {
+      assert BucketOf(g)
+          == map[]
+          == Compose(BucketOf(top), BucketOf(bot));
+    }*/
+  }
+
+  lemma GenFromBucketWithLowerBoundYieldsClampStart(bucket: Bucket, start: UI.RangeStart)
+  ensures var g := GenFromBucketWithLowerBound(bucket, start);
+      YieldsSortedBucket(g, ClampStart(bucket, start))
+  {
+    reveal_GenFromBucketWithLowerBound();
+    reveal_ClampStart();
+    reveal_BucketOf();
+
+    var g := GenFromBucketWithLowerBound(bucket, start);
+    var b1 := BucketOf(g);
+    var b2 := ClampStart(bucket, start);
+
+    //forall k | k in b1 ensures k in b2 && b2[k] == b1[k]
+    //{
+    //}
+
+    forall k | k in b2 ensures k in b1
+    {
+      match start {
+        case SExclusive(key) => {
+          noKeyBetweenIterFindFirstGt(bucket, key, k);
+        }
+        case SInclusive(key) => {
+          noKeyBetweenIterFindFirstGte(bucket, key, k);
+        }
+        case NegativeInf => {
+          noKeyBeforeIterStart(bucket, k);
+        }
+      }
+    }
+  }
+
+  lemma GenFromBucketStackWithLowerBoundYieldsComposeSeq(buckets: seq<Bucket>, start: UI.RangeStart)
+  requires |buckets| >= 1
+  ensures var g := GenFromBucketStackWithLowerBound(buckets, start);
+      YieldsSortedBucket(g, ClampStart(ComposeSeq(buckets), start))
+  {
+    reveal_GenFromBucketStackWithLowerBound();
+    var g := GenFromBucketStackWithLowerBound(buckets, start);
+    if |buckets| == 1 {
+      ComposeSeq1(buckets[0]);
+      assert [buckets[0]] == buckets;
+      GenFromBucketWithLowerBoundYieldsClampStart(buckets[0], start);
+    } else {
+      var mid := |buckets| / 2;
+      var g1 := GenFromBucketStackWithLowerBound(buckets[..mid], start);
+      var g2 := GenFromBucketStackWithLowerBound(buckets[mid..], start);
+      GenComposeIsCompose(g1, g2);
+      calc {
+        BucketOf(g);
+          { GenComposeIsCompose(g1, g2); }
+        Compose(BucketOf(g1), BucketOf(g2));
+          {
+            GenFromBucketStackWithLowerBoundYieldsComposeSeq(buckets[..mid], start);
+            GenFromBucketStackWithLowerBoundYieldsComposeSeq(buckets[mid..], start);
+          }
+        Compose(
+          ClampStart(ComposeSeq(buckets[..mid]), start), 
+          ClampStart(ComposeSeq(buckets[mid..]), start));
+          {
+            reveal_Compose();
+            reveal_ClampStart();
+          }
+        ClampStart(Compose(ComposeSeq(buckets[..mid]), ComposeSeq(buckets[mid..])), start);
+          { ComposeSeqAdditive(buckets[..mid], buckets[mid..]); }
+        ClampStart(ComposeSeq(buckets[..mid] + buckets[mid..]), start);
+          { assert buckets[..mid] + buckets[mid..] == buckets; }
+        ClampStart(ComposeSeq(buckets), start);
+      }
+    }
+  }
+
+  ////// For termination
+
+  function {:opaque} decreaser(g: Generator) : nat
+  requires WF(g)
+  {
+    match g {
+      case BasicGenerator(bucket, it) => (
+        it.decreaser
+      )
+      case ComposeGenerator(top, bot, next) => (
+        decreaser(top) + decreaser(bot) + (if next.Next? then 1 else 0)
+      )
+    }
+  }
+
+  lemma lemmaDecreaserDecreases(g: Generator)
+  requires WF(g)
+  ensures GenLeft(g).Next? ==> decreaser(GenPop(g)) < decreaser(g)
+  {
+    reveal_GenPop();
+    reveal_MergeGenPop();
+    reveal_BasicGenPop();
+    reveal_decreaser();
+    if g.ComposeGenerator? {
+      lemmaDecreaserDecreases(g.top);
+      lemmaDecreaserDecreases(g.bot);
+    }
+  }
+}
